proofs/trees.v
@@ -1,15 +1,16 @@
 From BalancedTrees Require Import definitions utils.
 
-Ltac get_couples :=
-  match goal with
-    | H: (_, _) = (_, _) |- _ => inversion H; subst end.
-
 Definition is_higher_rank (k1 : option A) (k2 : option A) : Prop :=
   match k1, k2 with
   | Some k1, Some k2 => (rank_of k2 < rank_of k1) \/ (rank_of k1 = rank_of k2 /\ k1 < k2)
-  | None, Some _ => True
-  | _, None => False
+  | Some _, _ => True
+  | None, _ => False
   end.
+
+Lemma is_higher_rank_than_none : forall k1, is_higher_rank (Some k1) None.
+Proof.
+  simpl. auto.
+Qed.
 
 Notation "k1 '≻' k2" := (is_higher_rank k1 k2) (at level 70).
 Notation "k1 '!≻' k2" := (is_higher_rank (Some k1) (Some k2)) (at level 70).
@@ -17,8 +18,8 @@ Notation "k1 '!≻' k2" := (is_higher_rank (Some k1) (Some k2)) (at level 70).
 Definition is_higher_rankb (k1: option A) (k2 : option A) : bool :=
   match k1, k2 with
   | Some k1, Some k2 => (rank_of k2 <? rank_of k1) || ((rank_of k1 =? rank_of k2) && (k1 <? k2))
-  | None, Some _ => true
-  | _, None => false
+  | Some _, None => true
+  | None, _ => false
   end.
 
 Notation "k1 '≻?' k2" := (is_higher_rankb k1 k2) (at level 70).
@@ -40,29 +41,19 @@ Lemma is_higher_rank_tricho : forall k k0,
     destruct (Nat.lt_trichotomy a a0) as [H0 | [H0 | H0]]; auto.
 Qed.
 
-Definition is_higher_rank_than_rootb (k : option A) (t: Tree) : bool :=
-  match t with
-  | Leaf => true
-  | Node _ k1 _ => k ≻? (Some k1)
-  end.
-
+(*Definition is_higher_rank_than_rootb (k : option A) (t: Tree) : bool :=
+  k ≻? root t.
+*)
 Definition is_higher_rank_than_root (k : option A) (t: Tree) : Prop :=
-  match t with
-  | Leaf => True
-  | Node _ k1 _ => k ≻ (Some k1)
-  end.
-
-Ltac get_root :=
-  match goal with
-    | H : is_higher_rank_than_root _ (Node _ _ _) |- _ => unfold is_higher_rank_than_root in H end.
+  k ≻ root t.
 
 Lemma is_higher_rank_than_root_trans : forall t x x0,
     is_higher_rank x0 x ->
     is_higher_rank_than_root x t ->
     is_higher_rank_than_root x0 t.
   intros. destruct x, x0; destruct t; auto.
-  - simpl. inversion H; inversion H0; intuition eauto using Nat.lt_trans; lia.
-  - inversion H.
+  - simpl in *. lia.
+  - simpl in *. tauto.
 Qed.
 
 Opaque is_higher_rank.
@@ -106,14 +97,43 @@ Inductive heap: Tree -> Prop :=
 
 Definition zip_tree (t: Tree) : Prop := heap t /\ abr t.
 
-#[local] Hint Rewrite app_assoc: app.
+
+
+Ltac get_couples :=
+  match goal with
+    | H: (_, _) = (_, _) |- _ => inversion H; subst; clear H end.
+
+Ltac get_root :=
+  match goal with
+  | H : is_higher_rank_than_root _ (Node _ _ _) |- _ => unfold is_higher_rank_than_root in H; simpl root in H end.
+
+Ltac get_heap :=
+  match goal with
+  | H : heap (Node _ _ _) |- _ => inversion H; subst end.
+
+Ltac simp_unzip_leaf :=
+  match goal with
+  | |- context [unzip Leaf _] => simp unzip end.
+
+Ltac simp_insert_leaf :=
+  match goal with
+  | |- context [insert Leaf _] => simp insert end.
+
+#[export] Hint Extern 0 => get_couples: core.
+#[export] Hint Extern 0 => get_root: core.
+#[export] Hint Extern 0 => get_heap: core.
+#[export] Hint Extern 0 => simp_unzip_leaf: core.
+#[export] Hint Extern 0 => simp_insert_leaf: core.
+#[export] Hint Unfold singleton_list is_higher_rank_than_root: core.
+#[export] Hint Immediate is_higher_rank_than_none: core.
+#[export] Hint Rewrite app_assoc: app.
 
 Lemma unzip_elts_occurs_k : forall t k a b, abr t ->
     unzip t k = (a, b) -> occurs k t ->
     elements t = elements a ++ [k] ++ elements b.
 Proof.
   intros t k. funelim (unzip t k); try easy.
-  - intros. subst. rewrite Nat.eqb_eq in *. subst. rewrite <- Heqcall in *. get_couples. auto.
+  - intros. subst. rewrite Nat.eqb_eq in *. subst. rewrite <- Heqcall in *. auto.
   - intros. rewrite <- Heqcall in *. get_couples. simp elements. autorewrite with app. repeat f_equal.
     rewrite <- app_assoc. apply abr_node in H1 as Habr. intuition. apply Hind; auto. apply Nat.ltb_lt in H0.
     eapply abr_lt_occurs; eauto.
@@ -127,8 +147,7 @@ Qed.
 Lemma unzip_elts_not_occurs_k : forall t k a b,
     abr t -> unzip t k = (a, b) -> ~ occurs k t -> elements t = elements a ++ elements b.
 Proof.
-  intros t k. funelim (unzip t k).
-  - simp unzip. intros. inversion H0. auto.
+  intros t k. funelim (unzip t k); auto.
   - intros. rewrite Nat.eqb_eq in *. subst. contradict H2. auto.
   - intros. rewrite <- Heqcall in *. get_couples. simp elements. autorewrite with app. repeat f_equal.
     apply abr_node in H1 as Habr. intuition. apply Hind; eauto.
@@ -165,7 +184,7 @@ Qed.
 Lemma unzip_smallers : forall t k a b, abr t -> unzip t k = (a, b) -> all_smallers a k.
 Proof.
   intros t k. funelim (unzip t k).
-  -  simp unzip. intros. inversion H0. subst. constructor.
+  -  simp unzip. intuition. intros. get_couples. constructor.
   - apply Nat.eqb_eq in H. subst. intros. apply abr_node in H. intuition. congruence.
   - intros. apply abr_node in H1. specialize (Hind st1 gt1). intuition. congruence.
   - intros. apply abr_node in H1. specialize (Hind st2 gt2). intuition. rewrite H2 in Heqcall. inversion Heqcall.
@@ -176,7 +195,7 @@ Qed.
 Lemma unzip_greaters : forall t k a b, abr t -> unzip t k = (a, b) -> all_greaters b k.
 Proof.
   intros t k. funelim (unzip t k).
-  -  simp unzip. intros. inversion H0. subst. constructor.
+  -  simp unzip. intros. get_couples. constructor.
   - apply Nat.eqb_eq in H. subst. intros. apply abr_node in H. intuition. congruence.
   - intros. apply abr_node in H1. specialize (Hind st1 gt1). intuition. rewrite H2 in Heqcall. inversion Heqcall.
     subst. unfold all_greaters. simp elements. apply Nat.ltb_lt in H0.
@@ -187,14 +206,13 @@ Qed.
 Lemma insert_elts : forall t k a b,
     abr t -> unzip t k = (a, b) -> elements (insert t k) = elements a ++ [k] ++ elements b.
 Proof.
-  intros t k. funelim (insert t k).
-  - simp unzip insert. intros. unfold singleton_list. inversion H0. auto.
-  - rewrite <- Heqcall. intros. simp elements. remember (unzip t2 k). destruct p. specialize (H t t0).
+  intros t k. funelim (insert t k); auto; rewrite <- Heqcall.
+  - intros. simp elements. remember (unzip t2 k). destruct p. specialize (H t t0).
     apply abr_node in H0 as Habr. intuition. rewrite H. simp unzip in H1. rewrite Nat.eqb_sym in *.
     apply ltb_neqb in Heq as Hneq. apply ltb_antisymm in Heq.
       rewrite Hneq, Heq in H1. simpl in H1. rewrite <- Heqp in H1. simpl in H1. get_couples. simp elements.
     repeat rewrite app_assoc. auto.
-  - rewrite <- Heqcall. intros. unfold is_higher_rankb in *. assert (kt =? k = false).
+  - intros. unfold is_higher_rankb in *. assert (kt =? k = false).
     + apply Nat.eqb_neq. intro. subst. apply orb_prop in Heq0. intuition.
       * rewrite Nat.ltb_irrefl in *. discriminate.
       * apply andb_prop in H2. intuition. rewrite Nat.ltb_irrefl in *. discriminate.
@@ -202,7 +220,7 @@ Proof.
       apply abr_node in H0 as Habr. intuition. rewrite H. simp unzip in H1. rewrite Nat.eqb_sym in H2.
       rewrite H2 in *. apply Nat.ltb_lt in Heq. rewrite Heq in H1. simpl in H1. rewrite <- Heqp in H1.
       simpl in H1. get_couples. simp elements. autorewrite with app. auto.
-  - rewrite <- Heqcall. rewrite Heq. simp elements. intros. inversion H0. subst. auto.
+  - rewrite Heq. simp elements. auto.
 Qed.
 
 Lemma insert_elts_set : forall t k x, abr t ->
@@ -240,15 +258,8 @@ Lemma unzip_preserves_is_higher_rank_than_root_fst : forall t k a b x,
     is_higher_rank_than_root x t ->
     is_higher_rank_than_root x a.
 Proof.
-  intros t k a b x. destruct x.
-  - funelim (unzip t k).
-    + simp unzip. intros. inversion H. auto.
-    + intros. inversion H1. apply Nat.eqb_eq in H. rewrite H0 in Heqcall. get_couples. get_root.
-      eauto using is_higher_rank_than_root_trans.
-    + rewrite <- Heqcall. intros. get_couples. specialize (Hind a gt1 a0). inversion H2. subst.
-      get_root. intuition eauto using is_higher_rank_than_root_trans.
-    + rewrite <- Heqcall. intros. inversion H1. intuition.
-  - intros. destruct a; constructor.
+  intros t k a b x. destruct x; auto.
+  funelim (unzip t k); auto; rewrite <- Heqcall; eauto using is_higher_rank_than_root_trans.
 Qed.
 
 Lemma unzip_preserves_is_higher_rank_than_root_snd : forall t k a b x,
@@ -257,35 +268,20 @@ Lemma unzip_preserves_is_higher_rank_than_root_snd : forall t k a b x,
     is_higher_rank_than_root x t ->
     is_higher_rank_than_root x b.
 Proof.
-  intros t k a b x. destruct x.
-  - funelim (unzip t k).
-    + simp unzip. intros. inversion H. auto.
-    + intros. inversion H1. apply Nat.eqb_eq in H. rewrite H0 in Heqcall. get_couples. get_root.
-      eauto using is_higher_rank_than_root_trans.
-    + rewrite <- Heqcall. intros. get_couples. auto.
-    + rewrite <- Heqcall. intros. get_couples. specialize (Hind st2 b a0). inversion H2. subst.
-      get_root. intuition eauto using is_higher_rank_than_root_trans.
-  - intros. destruct b; constructor.
+  intros t k a b x. destruct x; auto.
+  funelim (unzip t k); auto; rewrite <- Heqcall; eauto using is_higher_rank_than_root_trans.
 Qed.
 
 Lemma unzip_preserves_heap_fst : forall t k a b, unzip t k = (a, b) -> heap t -> heap a.
 Proof.
-  intros t k a b. funelim (unzip t k).
-  - simp unzip. intros. get_couples. auto.
-  - rewrite <- Heqcall. intros. get_couples. inversion H1. auto.
-  - rewrite <- Heqcall. intros. get_couples. specialize (Hind a gt1). inversion H2. intuition auto.
-  - rewrite <- Heqcall. intros. get_couples. specialize (Hind st2 b). inversion H2.
-    constructor; eauto using unzip_preserves_is_higher_rank_than_root_fst.
+  intros t k a b. funelim (unzip t k); auto; rewrite <- Heqcall;
+    intuition eauto 6 using heap, unzip_preserves_is_higher_rank_than_root_fst.
 Qed.
 
 Lemma unzip_preserves_heap_snd : forall t k a b, unzip t k = (a, b) -> heap t -> heap b.
 Proof.
-  intros t k a b. funelim (unzip t k).
-  - simp unzip. intros. inversion H. auto.
-  - rewrite <- Heqcall. intros. get_couples. inversion H1. auto.
-  - rewrite <- Heqcall. intros. get_couples. specialize (Hind a gt1). inversion H2.
-    constructor; eauto using unzip_preserves_is_higher_rank_than_root_snd.
-  - rewrite <- Heqcall. intros. get_couples. specialize (Hind st2 b). inversion H2. intuition auto.
+  intros t k a b. funelim (unzip t k); auto; rewrite <- Heqcall;
+    intuition eauto 6 using heap, unzip_preserves_is_higher_rank_than_root_snd.
 Qed.
 
 Lemma insert_preserves_is_higher_rank_than_root : forall t k x,
@@ -293,32 +289,27 @@ Lemma insert_preserves_is_higher_rank_than_root : forall t k x,
     is_higher_rank x (Some k) ->
     is_higher_rank_than_root x (insert t k).
 Proof.
-  unfold is_higher_rank_than_root. intros. destruct x.
-  - destruct t.
-    + simp insert. auto.
-    + simp insert. remember (a0 !≻? k). destruct b; simpl.
-      * apply eq_sym, is_higher_rank_dec in Heqb. destruct (a0 <? k); simpl; auto.
-      * destruct (unzip (Node t1 a0 t2) k). simpl. auto.
+  intros. destruct x.
+  - destruct t; auto. simp insert. remember (a0 !≻? k). destruct b; simpl.
+    + apply eq_sym, is_higher_rank_dec in Heqb. destruct (a0 <? k); simpl; auto.
+    + destruct (unzip (Node t1 a0 t2) k). auto.
   - destruct (insert t k); auto.
 Qed.
 
 Lemma insert_preserves_heap : forall t k, heap t -> heap (insert t k).
-  intros t k. funelim (insert t k).
-  - simp insert. constructor; simpl; auto.
-  - intro. inversion H0. subst. intuition. rewrite <- Heqcall. apply is_higher_rank_dec in Heq0.
-    constructor; auto using insert_preserves_is_higher_rank_than_root.
-  - intro. inversion H0. subst. intuition. rewrite <- Heqcall. apply is_higher_rank_dec in Heq0.
-    constructor; auto using insert_preserves_is_higher_rank_than_root.
-  - intro H0.  inversion H0. subst. intuition. rewrite <- Heqcall. 
-    constructor; eauto using unzip_preserves_heap_fst, unzip_preserves_heap_snd.
-    + destruct (is_higher_rank_tricho (Some kt) (Some k)) as [Hrank | [Hrank | Hrank]].
+  intros t k. funelim (insert t k); eauto using heap.
+  - rewrite <- Heqcall. apply is_higher_rank_dec in Heq0.
+    eauto using heap, insert_preserves_is_higher_rank_than_root.    
+  - rewrite <- Heqcall. apply is_higher_rank_dec in Heq0.
+    eauto using heap, insert_preserves_is_higher_rank_than_root.
+  - intro H0. get_heap. rewrite <- Heqcall.
+    constructor; eauto using unzip_preserves_heap_fst, unzip_preserves_heap_snd;
+      destruct (is_higher_rank_tricho (Some kt) (Some k)) as [ Hrank | [Hrank | Hrank]];
+      eauto using unzip_preserves_is_higher_rank_than_root_fst, unzip_preserves_is_higher_rank_than_root_snd.
       * apply is_higher_rank_dec in Hrank. congruence.
-      * inversion Hrank. subst. simp unzip in Heq. rewrite Nat.eqb_refl in Heq. simpl in Heq. get_couples. auto.
-      * eauto using unzip_preserves_is_higher_rank_than_root_fst.
-    + destruct (is_higher_rank_tricho (Some kt) (Some k)) as [Hrank | [Hrank | Hrank]].
+      * inversion Hrank. subst. simp unzip in Heq. rewrite Nat.eqb_refl in Heq. simpl in Heq. auto.
       * apply is_higher_rank_dec in Hrank. congruence.
-      * inversion Hrank. subst. simp unzip in Heq. rewrite Nat.eqb_refl in Heq. simpl in Heq. get_couples. auto.
-      * eauto using unzip_preserves_is_higher_rank_than_root_snd.
+      * inversion Hrank. subst. simp unzip in Heq. rewrite Nat.eqb_refl in Heq. simpl in Heq. auto.
 Qed.
 
 Theorem insert_correct : forall t k,
